LeanCats/HashMapExt.lean
@@ -1,0 +1,35 @@
+import Std.Data.HashMap
+import Lean
+
+open Lean
+open Std
+
+-- HashMap Extention:
+-- Copied from https://leanprover.zulipchat.com/#narrow/channel/270676-lean4/topic/HashMap.20extension
+def HashMapExtension (α β : Type) [BEq α] [Hashable α] := SimplePersistentEnvExtension (α × β) (HashMap α β)
+
+instance (α β : Type) [BEq α] [Hashable α] : Inhabited (HashMapExtension α β) :=
+  inferInstanceAs (Inhabited (SimplePersistentEnvExtension (α × β) (HashMap α β)))
+
+def mkHashMapExtension (name : Name) (α β : Type) [BEq α] [Hashable α]  : IO (HashMapExtension α β) :=
+  registerSimplePersistentEnvExtension {
+    name          := name,
+    addImportedFn := mkStateFromImportedEntries (λ s n => s.insert n.1 n.2) {},
+    addEntryFn    := (λ s n => s.insert n.1 n.2),
+    toArrayFn     := fun es => es.toArray
+  }
+
+namespace HashMapExtension
+
+variable {α β : Type} [BEq α] [Hashable α] {m: Type → Type} [Monad m] [MonadEnv m]
+
+def find? (ext : HashMapExtension α β) (a : α) : m $ Option β := do
+  return (ext.getState (← getEnv)).get? a
+
+def insert (ext : HashMapExtension α β) (a : α) (b : β) : m Unit :=
+  modifyEnv (ext.addEntry · (a, b))
+
+def update (ext : HashMapExtension α β) (a : α) (b : β) : m Unit :=
+  modifyEnv (ext.addEntry · (a, b))
+
+end HashMapExtension
