lakefile.lean
@@ -15,3 +15,6 @@ lean_exe "test-to-string" where
   root := `LeanCats.TestToString
 
 require "leanprover-community" / "mathlib"
+
+-- You should replace v0.0.3 with the latest version published under Releases
+require proofwidgets from git "https://github.com/leanprover-community/ProofWidgets4"@"v0.0.90"
